Types.dfy
@@ -1,0 +1,490 @@
+include "Auxiliary.dfy"
+
+module TypeMod{
+  /*type A(==)
+  type B(==)
+  type C(==)
+  type D(==)
+  type T(==)*/
+  const sizeT:nat := 1  // upper bound
+  const upperBound:nat    // hacer TypeMod abstract?
+  //function polynomial() : nat
+
+
+  type Set<T(==)>{
+
+  ghost function Model():set<T>
+  ghost function Size():nat
+  {|Model()|*sizeT}
+
+  method Pick(ghost counter_in:nat) returns (e:T, ghost counter_out:nat)
+    requires Model() != {}
+    ensures counter_out == counter_in + sizeT
+    ensures e in Model()
+  
+  method Empty(ghost counter_in:nat) returns (b:bool, ghost counter_out:nat)
+    ensures b == (Model() == {})
+    ensures counter_out == counter_in + 1
+  
+  method Cardinality(ghost counter_in:nat) returns (size:int, ghost counter_out:nat)
+    ensures  size == |Model()|
+    ensures counter_out == counter_in + 1
+  
+  method Add(e:T, ghost counter_in:nat) returns (R:Set<T>, ghost counter_out:nat)
+    ensures  R.Model() == Model() + {e}
+    ensures if e in Model() then |R.Model()| == |Model()|
+            else |R.Model()| == |Model()| + 1
+    ensures counter_out == counter_in + sizeT
+
+  method Remove(e:T, ghost counter_in:nat) returns (R:Set<T>, ghost counter_out:nat)
+    ensures  R.Model() == Model() - {e}
+    ensures if e !in Model() then |R.Model()| == |Model()|
+            else |R.Model()| == |Model()| - 1
+    ensures counter_out == counter_in + Size()
+  
+  method Contains(e:T, ghost counter_in:nat) returns (b:bool, ghost counter_out:nat)
+    ensures  b == (e in Model()) 
+    ensures counter_out == counter_in + Size()
+
+  method Copy(ghost counter_in:nat) returns (R:Set<T>, ghost counter_out:nat)
+    ensures R.Model() == Model()
+    ensures counter_out == counter_in + Size()
+
+  }
+
+
+  type SetSet<T(==)>{
+   ghost function Model():set<set<T>>
+   ghost function maximumSizeElements():nat
+   ensures forall s | s in Model() :: maximumSizeElements() >= |s|*sizeT
+   ensures exists s :: s in Model() && maximumSizeElements() == |s|*sizeT
+
+   ghost function Size():nat
+    {|Model()|*maximumSizeElements()}
+
+  method Pick(ghost counter_in:nat) returns (e:Set<T>, ghost counter_out:nat)
+    requires Model() != {}
+    ensures counter_out == counter_in + maximumSizeElements()
+    ensures e.Model() in Model()
+
+  method Empty(ghost counter_in:nat) returns (b: bool, ghost counter_out:nat)
+    ensures b == (Model() == {})
+    ensures counter_out == counter_in + 1
+  
+  method Cardinality(ghost counter_in:nat) returns (size: int, ghost counter_out:nat)
+    ensures  size == |Model()|
+    ensures counter_out == counter_in + 1
+  
+  method Add(e:Set<T>, ghost counter_in:nat) returns (R:SetSet<T>, ghost counter_out:nat)
+    ensures  R.Model() == Model() + {e.Model()}
+    ensures if e.Model() in Model() then |R.Model()| == |Model()|
+            else |R.Model()| == |Model()| + 1
+    ensures counter_out == counter_in + maximumSizeElements()
+
+  method Remove(e:Set<T>, ghost counter_in:nat) returns (R:SetSet<T>, ghost counter_out:nat)
+    ensures  R.Model() == Model() - {e.Model()}
+    ensures if e.Model() !in Model() then |R.Model()| == |Model()|
+            else |R.Model()| == |Model()| - 1
+    ensures counter_out == counter_in + Size()
+  
+  method Contains(e:Set<T>, ghost counter_in:nat) returns (b:bool, ghost counter_out:nat)
+    ensures  b == (e.Model() in Model()) 
+    ensures counter_out == counter_in + Size()
+
+  method Copy(ghost counter_in:nat) returns (R:SetSet<T>, ghost counter_out:nat)
+    ensures R.Model() == Model()
+    ensures counter_out == counter_in + Size()
+  }
+
+
+  type SetSetSet<T(==)>{
+   ghost function Model():set<set<set<T>>>
+
+   ghost function maximumSizeElements():nat
+   ensures forall s | s in Model() :: maximumSizeElements() >= |s|*maximumSizeElements'()
+   ensures exists s :: s in Model() && maximumSizeElements() == |s|*maximumSizeElements'()
+
+   ghost function maximumSizeElements'():nat
+   ensures forall s | s in Model() :: (forall s' | s' in s :: maximumSizeElements'() >= |s'|*sizeT)
+   ensures exists s | s in Model() :: (exists s' | s' in s :: maximumSizeElements'() == |s'|*sizeT)
+
+
+   ghost function Size():nat
+    {|Model()|*maximumSizeElements()}
+
+  method Pick(ghost counter_in:nat) returns (e:SetSet<T>, ghost counter_out:nat)
+    requires Model() != {}
+    ensures counter_out == counter_in + maximumSizeElements()
+    ensures e.Model() in Model()
+
+  method Empty(ghost counter_in:nat) returns (b: bool, ghost counter_out:nat)
+    ensures b == (Model() == {})
+    ensures counter_out == counter_in + 1
+  
+  method Cardinality(ghost counter_in:nat) returns (size: int, ghost counter_out:nat)
+    ensures  size == |Model()|
+    ensures counter_out == counter_in + 1
+  
+  method Add(e:SetSet<T>, ghost counter_in:nat) returns (R:SetSetSet<T>, ghost counter_out:nat)
+    ensures  R.Model() == Model() + {e.Model()}
+    ensures if e.Model() in Model() then |R.Model()| == |Model()|
+            else |R.Model()| == |Model()| + 1
+    ensures counter_out == counter_in + maximumSizeElements()
+
+  method Remove(e:SetSet<T>, ghost counter_in:nat) returns (R:SetSetSet<T>, ghost counter_out:nat)
+    ensures  R.Model() == Model() - {e.Model()}
+    ensures if e.Model() !in Model() then |R.Model()| == |Model()|
+            else |R.Model()| == |Model()| - 1
+    ensures counter_out == counter_in + Size()
+  
+  method Contains(e:SetSet<T>, ghost counter_in:nat) returns (b:bool, ghost counter_out:nat)
+    ensures  b == (e.Model() in Model()) 
+    ensures counter_out == counter_in + Size()
+
+  method Copy(ghost counter_in:nat) returns (R:SetSetSet<T>, ghost counter_out:nat)
+    ensures R.Model() == Model()
+    ensures counter_out == counter_in + Size()
+  }
+
+
+  type Map<T0(==), T1(==)>{
+
+  ghost function Model():map<T0, T1>
+  ghost function Size():nat
+  {|Model()|*sizeT}
+
+  method Get(q:T0, ghost counter_in:nat) returns (a:T1, ghost counter_out:nat)
+    requires Model() != map[]
+    requires q in Model().Keys
+    ensures counter_out == counter_in + sizeT
+    ensures a == Model()[q]
+
+  method Add(q:T0, a:T1, ghost counter_in:nat) returns (R:Map<T0, T1>, ghost counter_out:nat)
+    //requires !(q in Model().Keys)
+    ensures counter_out == counter_in + sizeT
+    ensures R.Model() == Model()[q := a]
+
+  method Remove(q:T0, ghost counter_in:nat) returns (R:Map<T0, T1>, ghost counter_out:nat)
+    requires q in Model().Keys
+    ensures counter_out == counter_in + sizeT
+    ensures R.Model() == Model() - {q}
+
+  method Keys(ghost counter_in:nat) returns (keys:Set<T0>, ghost counter_out:nat)
+    ensures counter_out == counter_in + Size()
+    ensures keys.Model() == Model().Keys
+
+  method Values(ghost counter_in:nat) returns (keys:Set<T1>, ghost counter_out:nat)
+    ensures counter_out == counter_in + Size()
+    ensures keys.Model() == Model().Values
+
+  method Items(ghost counter_in:nat) returns (keys:Set<(T0, T1)>, ghost counter_out:nat)
+    ensures counter_out == counter_in + Size()
+    ensures keys.Model() == Model().Items
+
+  method HasKey(q:T0, ghost counter_in:nat) returns (b:bool, ghost counter_out:nat)
+    ensures counter_out == counter_in + sizeT
+    ensures b == (q in Model().Keys)
+  
+  /*
+  method Restrict(s:set<T0>, ghost counter_in:nat) returns (R:map<T0, T1>, ghost counter_out:nat)
+    requires s <= Model().Keys
+    ensures counter_out == counter_in + Size()
+    ensures R.Keys == s
+    ensures forall key:T0 | key in R.Keys :: R[key] == Model()[key]
+    ensures forall i:(T0, T1) | i in R.Items :: i in Model().Items              // redundante
+  */
+  
+  }
+
+
+  type MapMap<T0(==), T1(==), T2(==)>{
+
+  ghost function Model():map<map<T0, T1>, T2>
+  ghost function Size():nat
+  {|Model()|*maximumSizeElements()}
+
+   ghost function maximumSizeElements():nat
+   ensures forall s | s in Model().Keys :: maximumSizeElements() >= |s.Items|*sizeT
+   ensures exists s :: s in Model() && maximumSizeElements() == |s.Items|*sizeT
+
+  method Get(q:Map<T0, T1>, ghost counter_in:nat) returns (a:T2, ghost counter_out:nat)
+    requires Model() != map[]
+    requires q.Model() in Model().Keys
+    ensures counter_out == counter_in + maximumSizeElements()
+    ensures a == Model()[q.Model()]
+
+  method Add(q:Map<T0, T1>, a:T2, ghost counter_in:nat) returns (R:MapMap<T0, T1, T2>, ghost counter_out:nat)
+    //requires !(q in Model().Keys)
+    ensures counter_out == counter_in + maximumSizeElements()
+    ensures R.Model() == Model()[q.Model() := a]
+  
+  method Remove(q:Map<T0, T1>, ghost counter_in:nat) returns (R:MapMap<T0, T1, T2>, ghost counter_out:nat)
+      requires q.Model() in Model().Keys
+      ensures counter_out == counter_in + maximumSizeElements()
+      ensures R.Model() == Model() - {q.Model()}
+    
+  method Keys(ghost counter_in:nat) returns (keys:SetMap<T0, T1>, ghost counter_out:nat)
+    ensures counter_out == counter_in + Size()
+    ensures keys.Model() == Model().Keys
+
+  method Values(ghost counter_in:nat) returns (keys:Set<T2>, ghost counter_out:nat)
+    ensures counter_out == counter_in + Size()
+    ensures keys.Model() == Model().Values
+
+  method Items(ghost counter_in:nat) returns (keys:SetPairMap<T0, T1, T2>, ghost counter_out:nat)
+    ensures counter_out == counter_in + Size()
+    ensures keys.Model() == Model().Items
+
+  method HasKey(q:Map<T0, T1>, ghost counter_in:nat) returns (b:bool, ghost counter_out:nat)
+    ensures counter_out == counter_in + sizeT
+    ensures b == (q.Model() in Model().Keys)
+
+  }
+  
+
+  type Map_Map_SetMap<T0(==), T1(==)>{
+
+  ghost function Model():map<map<T0, T1>, set<map<T0, T1>>>
+  ghost function Size():nat
+  {|Model()|*maximumSizeElements()}
+
+  ghost function maximumSizeElements():nat
+  ensures ((maximumSizeElements() >= maximumSizeKeys()) && (maximumSizeElements() == maximumSizeValues())) ||
+          ((maximumSizeElements() == maximumSizeKeys()) && (maximumSizeElements() >= maximumSizeValues()))
+
+  ghost function maximumSizeKeys():nat
+  ensures forall s | s in Model().Keys :: maximumSizeKeys() >= |s.Items|*sizeT
+  ensures exists s :: s in Model() && maximumSizeKeys() == |s.Items|*sizeT
+
+  ghost function maximumSizeValues():nat
+  ensures forall setMap | setMap in Model().Values ::
+          forall m | m in setMap :: maximumSizeValues() >= |m.Items|*sizeT
+  ensures exists setMap | setMap in Model().Values ::
+          exists m | m in setMap :: maximumSizeValues() == |m.Items|*sizeT
+
+  method Get(q:Map<T0, T1>, ghost counter_in:nat) returns (a:SetMap<T0, T1>, ghost counter_out:nat)
+    requires Model() != map[]
+    requires q.Model() in Model().Keys
+    ensures counter_out == counter_in + maximumSizeElements()
+    ensures a.Model() == Model()[q.Model()]
+
+  method Add(q:Map<T0, T1>, a:SetMap<T0, T1>, ghost counter_in:nat) returns (R:Map_Map_SetMap<T0, T1>, ghost counter_out:nat)
+    //requires !(q in Model().Keys)
+    ensures counter_out == counter_in + maximumSizeElements()
+    ensures R.Model() == Model()[q.Model() := a.Model()]
+  
+  method Remove(q:Map<T0, T1>, ghost counter_in:nat) returns (R:Map_Map_SetMap<T0, T1>, ghost counter_out:nat)
+      requires q.Model() in Model().Keys
+      ensures counter_out == counter_in + maximumSizeElements()
+      ensures R.Model() == Model() - {q.Model()}
+    
+  method Keys(ghost counter_in:nat) returns (keys:SetMap<T0, T1>, ghost counter_out:nat)
+    ensures counter_out == counter_in + Size()
+    ensures keys.Model() == Model().Keys
+
+  method Values(ghost counter_in:nat) returns (keys:SetSetMap<T0, T1>, ghost counter_out:nat)
+    ensures counter_out == counter_in + Size()
+    ensures keys.Model() == Model().Values
+
+  method HasKey(q:Map<T0, T1>, ghost counter_in:nat) returns (b:bool, ghost counter_out:nat)
+    ensures counter_out == counter_in + sizeT
+    ensures b == (q.Model() in Model().Keys)
+
+  }
+  
+
+  type SetMap<T0(==), T1(==)>{
+    ghost function Model():set<map<T0, T1>>
+
+    ghost function Size():nat
+    {|Model()|*maximumSizeElements()}
+
+    ghost function maximumSizeElements():nat
+    ensures forall s | s in Model() :: maximumSizeElements() >= |s.Items|*sizeT
+    ensures exists s :: s in Model() && maximumSizeElements() == |s.Items|*sizeT
+
+    method Pick(ghost counter_in:nat) returns (e:Map<T0, T1>, ghost counter_out:nat)
+      requires Model() != {}
+      ensures counter_out == counter_in + maximumSizeElements()
+      ensures e.Model() in Model()
+    
+    method Empty(ghost counter_in:nat) returns (b:bool, ghost counter_out:nat)
+      ensures b == (Model() == {})
+      ensures counter_out == counter_in + 1
+    
+    method Cardinality(ghost counter_in:nat) returns (size: int, ghost counter_out:nat)
+      ensures  size == |Model()|
+      ensures counter_out == counter_in + 1
+    
+    method Add(e:Map<T0, T1>, ghost counter_in:nat) returns (R:SetMap<T0, T1>, ghost counter_out:nat)
+      ensures  R.Model() == Model() + {e.Model()}
+      ensures if e.Model() in Model() then |R.Model()| == |Model()|
+              else |R.Model()| == |Model()| + 1
+      ensures counter_out == counter_in + Size()
+
+    method Remove(e:Map<T0, T1>, ghost counter_in:nat) returns (R:SetMap<T0, T1>, ghost counter_out:nat)
+      ensures  R.Model() == Model() - {e.Model()}
+      ensures if e.Model() !in Model() then |R.Model()| == |Model()|
+              else |R.Model()| == |Model()| - 1
+      ensures counter_out == counter_in + Size()
+    
+    method Contains(e:Map<T0, T1>, ghost counter_in:nat) returns (b:bool, ghost counter_out:nat)
+      ensures  b == (e.Model() in Model()) 
+      ensures counter_out == counter_in + Size()
+
+    method Copy(ghost counter_in:nat) returns (R:SetMap<T0, T1>, ghost counter_out:nat)
+      ensures R.Model() == Model()
+      ensures counter_out == counter_in + Size()
+
+  }
+
+
+type SetSetMap<T0(==), T1(==)>{
+    ghost function Model():set<set<map<T0, T1>>>
+
+    ghost function Size():nat
+    {|Model()|*maximumSizeElements()}
+
+    ghost function maximumSizeElements():nat
+    // ensures forall s | s in Model() :: maximumSizeElements() >= |s.Items|*sizeT
+    //ensures exists s :: s in Model() && maximumSizeElements() == |s.Items|*sizeT
+
+    method Pick(ghost counter_in:nat) returns (e:SetMap<T0, T1>, ghost counter_out:nat)
+      requires Model() != {}
+      ensures counter_out == counter_in + maximumSizeElements()
+      ensures e.Model() in Model()
+    
+    method Empty(ghost counter_in:nat) returns (b:bool, ghost counter_out:nat)
+      ensures b == (Model() == {})
+      ensures counter_out == counter_in + 1
+    
+    method Cardinality(ghost counter_in:nat) returns (size: int, ghost counter_out:nat)
+      ensures  size == |Model()|
+      ensures counter_out == counter_in + 1
+    
+    method Add(e:SetMap<T0, T1>, ghost counter_in:nat) returns (R:SetSetMap<T0, T1>, ghost counter_out:nat)
+      ensures  R.Model() == Model() + {e.Model()}
+      ensures if e.Model() in Model() then |R.Model()| == |Model()|
+              else |R.Model()| == |Model()| + 1
+      ensures counter_out == counter_in + Size()
+
+    method Remove(e:SetMap<T0, T1>, ghost counter_in:nat) returns (R:SetSetMap<T0, T1>, ghost counter_out:nat)
+      ensures  R.Model() == Model() - {e.Model()}
+      ensures if e.Model() !in Model() then |R.Model()| == |Model()|
+              else |R.Model()| == |Model()| - 1
+      ensures counter_out == counter_in + Size()
+    
+    method Contains(e:SetMap<T0, T1>, ghost counter_in:nat) returns (b:bool, ghost counter_out:nat)
+      ensures  b == (e.Model() in Model()) 
+      ensures counter_out == counter_in + Size()
+
+    method Copy(ghost counter_in:nat) returns (R:SetSetMap<T0, T1>, ghost counter_out:nat)
+      ensures R.Model() == Model()
+      ensures counter_out == counter_in + Size()
+
+  }
+
+
+  type SetPairMap<T0(==), T1(==), T2(==)>{
+    ghost function Model():set<(map<T0, T1>, T2)>
+
+    ghost function Size():nat
+    {|Model()|*maximumSizeElements()}
+
+    ghost function maximumSizeElements():nat
+    ensures forall s | s in Model() :: maximumSizeElements() >= |s.0.Items|*sizeT
+    ensures exists s :: s in Model() && maximumSizeElements() == |s.0.Items|*sizeT
+
+    method Pick(ghost counter_in:nat) returns (e:(Map<T0, T1>, T2), ghost counter_out:nat)
+      requires Model() != {}
+      ensures counter_out == counter_in + maximumSizeElements()
+      ensures exists m | m in Model() :: m.0 == e.0.Model() && m.1 == e.1
+    
+    method Empty(ghost counter_in:nat) returns (b:bool, ghost counter_out:nat)
+      ensures b == (Model() == {})
+      ensures counter_out == counter_in + 1
+    
+    method Cardinality(ghost counter_in:nat) returns (size: int, ghost counter_out:nat)
+      ensures  size == |Model()|
+      ensures counter_out == counter_in + 1
+    
+    method Add(e:(Map<T0, T1>, T2), ghost counter_in:nat) returns (R:SetPairMap<T0, T1, T2>, ghost counter_out:nat)
+      ensures  R.Model() == Model() + {(e.0.Model(), e.1)}
+      ensures if (e.0.Model(), e.1) in Model() then |R.Model()| == |Model()|
+              else |R.Model()| == |Model()| + 1
+      ensures counter_out == counter_in + Size()
+
+    method Remove(e:(Map<T0, T1>, T2), ghost counter_in:nat) returns (R:SetPairMap<T0, T1, T2>, ghost counter_out:nat)
+      ensures  R.Model() == Model() - {(e.0.Model(), e.1)}
+      ensures if (e.0.Model(), e.1) !in Model() then |R.Model()| == |Model()|
+              else |R.Model()| == |Model()| - 1
+      ensures counter_out == counter_in + Size()
+    
+    method Contains(e:(Map<T0, T1>, T2), ghost counter_in:nat) returns (b:bool, ghost counter_out:nat)
+      ensures  b == ((e.0.Model(), e.1) in Model()) 
+      ensures counter_out == counter_in + Size()
+
+    method Copy(ghost counter_in:nat) returns (R:SetPairMap<T0, T1, T2>, ghost counter_out:nat)
+      ensures R.Model() == Model()
+      ensures counter_out == counter_in + Size()
+
+  }
+
+
+ method NewSet(ghost counter_in:nat) returns (R:Set, ghost counter_out:nat)
+    ensures counter_out == counter_in +1
+    ensures R.Model() == {}
+  
+  method NewSetSet(ghost counter_in:nat) returns (R:SetSet, ghost counter_out:nat)
+    ensures counter_out == counter_in +1
+    ensures R.Model() == {}
+
+  method NewSetSetSet(ghost counter_in:nat) returns (R:SetSetSet, ghost counter_out:nat)
+    ensures counter_out == counter_in +1
+    ensures R.Model() == {}
+
+  method MakeSet<T(==)>(s:set<T>, ghost sizeT:nat, ghost counter_in:nat) returns (R:Set, ghost counter_out:nat)
+    ensures counter_out == counter_in + sizeT*|s|
+    ensures R.Model() == s
+
+
+  method NewMap(ghost counter_in:nat) returns (R:Map, ghost counter_out:nat)
+    ensures counter_out == counter_in +1
+    ensures R.Model() == map[]
+
+  method NewMapMap(ghost counter_in:nat) returns (R:MapMap, ghost counter_out:nat)
+    ensures counter_out == counter_in +1
+    ensures R.Model() == map[]
+
+  method MakeMap<A(==), B(==)>(s:map<A, B>, ghost sizeT:nat, ghost counter_in:nat) returns (R:Map<A, B>, ghost counter_out:nat)
+    ensures counter_out == counter_in + sizeT*|s|
+    ensures R.Model() == s
+
+
+}
+
+
+
+/*
+module IntMod refines TypeMod {
+  type T = int
+  const sizeT := 1
+}
+
+module BoolMod refines TypeMod {
+  type T = bool
+  const sizeT := 1
+}
+
+module QuestionMod refines TypeMod {
+  import opened Auxiliary
+  type T = Question
+  const sizeT := 1
+}
+
+module AnswerMod refines TypeMod {
+  import opened Auxiliary
+  type T = Answer
+  const sizeT := 1
+}
+*/
